Use SProp for Pmap and gmap sigma types

theories/gmap.v
@@ -20,8 +20,8 @@ Unset Default Proof Using.
 (** * The data structure *)
 (** We pack a [Pmap] together with a proof that ensures that all keys correspond
 to codes of actual elements of the countable type. *)
-Definition gmap_wf K `{Countable K} {A} (m : Pmap A) : Prop :=
-  bool_decide (map_Forall (λ p _, encode (A:=K) <$> decode p = Some p) m).
+Definition gmap_wf K `{Countable K} {A} (m : Pmap A) : SProp :=
+  sprop_decide (map_Forall (λ p _, encode (A:=K) <$> decode p = Some p) m).
 Record gmap K `{Countable K} A := GMap {
   gmap_car : Pmap A;
   gmap_prf : gmap_wf K gmap_car
@@ -31,8 +31,7 @@ Global Arguments gmap_car {_ _ _ _} _ : assert.
 Lemma gmap_eq `{Countable K} {A} (m1 m2 : gmap K A) :
   m1 = m2 ↔ gmap_car m1 = gmap_car m2.
 Proof.
-  split; [by intros ->|intros]. destruct m1, m2; simplify_eq/=.
-  f_equal; apply proof_irrel.
+  split; [by intros ->|intros]. destruct m1, m2; simplify_eq/=; done.
 Qed.
 Global Instance gmap_eq_eq `{Countable K, EqDecision A} : EqDecision (gmap K A).
 Proof.
@@ -43,7 +42,7 @@ Defined.
 (** * Operations on the data structure *)
 Global Instance gmap_lookup `{Countable K} {A} : Lookup K A (gmap K A) :=
   λ i '(GMap m _), m !! encode i.
-Global Instance gmap_empty `{Countable K} {A} : Empty (gmap K A) := GMap ∅ I.
+Global Instance gmap_empty `{Countable K} {A} : Empty (gmap K A) := GMap ∅ stt.
 (** Block reduction, even on concrete [gmap]s.
 Marking [gmap_empty] as [simpl never] would not be enough, because of
 https://github.com/coq/coq/issues/2972 and
@@ -55,7 +54,7 @@ Global Opaque gmap_empty.
 Lemma gmap_partial_alter_wf `{Countable K} {A} (f : option A → option A) m i :
   gmap_wf K m → gmap_wf K (partial_alter f (encode (A:=K) i) m).
 Proof.
-  unfold gmap_wf; rewrite !bool_decide_spec.
+  unfold gmap_wf; apply is_true_fmap; rewrite !bool_decide_spec.
   intros Hm p x. destruct (decide (encode i = p)) as [<-|?].
   - rewrite decode_encode; eauto.
   - rewrite lookup_partial_alter_ne by done. by apply Hm.
@@ -68,7 +67,7 @@ Global Instance gmap_partial_alter `{Countable K} {A} :
 Lemma gmap_fmap_wf `{Countable K} {A B} (f : A → B) m :
   gmap_wf K m → gmap_wf K (f <$> m).
 Proof.
-  unfold gmap_wf; rewrite !bool_decide_spec.
+  unfold gmap_wf; apply is_true_fmap; rewrite !bool_decide_spec.
   intros ? p x. rewrite lookup_fmap, fmap_Some; intros (?&?&?); eauto.
 Qed.
 Global Instance gmap_fmap `{Countable K} : FMap (gmap K) := λ A B f '(GMap m Hm),
@@ -76,7 +75,7 @@ Global Instance gmap_fmap `{Countable K} : FMap (gmap K) := λ A B f '(GMap m Hm
 Lemma gmap_omap_wf `{Countable K} {A B} (f : A → option B) m :
   gmap_wf K m → gmap_wf K (omap f m).
 Proof.
-  unfold gmap_wf; rewrite !bool_decide_spec.
+  unfold gmap_wf; apply is_true_fmap; rewrite !bool_decide_spec.
   intros ? p x; rewrite lookup_omap, bind_Some; intros (?&?&?); eauto.
 Qed.
 Global Instance gmap_omap `{Countable K} : OMap (gmap K) := λ A B f '(GMap m Hm),
@@ -85,8 +84,11 @@ Lemma gmap_merge_wf `{Countable K} {A B C}
     (f : option A → option B → option C) m1 m2 :
   gmap_wf K m1 → gmap_wf K m2 → gmap_wf K (merge f m1 m2).
 Proof.
-  unfold gmap_wf; rewrite !bool_decide_spec.
-  intros Hm1 Hm2 p z. rewrite lookup_merge; intros.
+  unfold gmap_wf.
+  refine (λ H1' H2', is_true_bind H1' (λ H1, is_true_bind H2' (λ H2, is_true_intro (_ H1 H2)))).
+  clear H1 H2 H1' H2'.
+  rewrite !bool_decide_spec.
+  intros Hm1 Hm2 p z; rewrite lookup_merge by done; intros.
   destruct (m1 !! _) eqn:?, (m2 !! _) eqn:?; naive_solver.
 Qed.
 Global Instance gmap_merge `{Countable K} : Merge (gmap K) :=
@@ -102,7 +104,7 @@ Proof.
   split.
   - unfold lookup; intros A [m1 Hm1] [m2 Hm2] Hm.
     apply gmap_eq, map_eq; intros i; simpl in *.
-    apply bool_decide_unpack in Hm1; apply bool_decide_unpack in Hm2.
+    apply sprop_decide_unpack in Hm1; apply sprop_decide_unpack in Hm2.
     apply option_eq; intros x; split; intros Hi.
     + pose proof (Hm1 i x Hi); simpl in *.
       by destruct (decode i); simplify_eq/=; rewrite <-Hm.
@@ -114,7 +116,7 @@ Proof.
     by contradict Hs; apply (inj encode).
   - intros A B f [m Hm] i; apply (lookup_fmap f m).
   - intros A [m Hm]; unfold map_to_list; simpl.
-    apply bool_decide_unpack, map_Forall_to_list in Hm; revert Hm.
+    apply sprop_decide_unpack, map_Forall_to_list in Hm; revert Hm.
     induction (NoDup_map_to_list m) as [|[p x] l Hpx];
       inversion 1 as [|??? Hm']; simplify_eq/=; [by constructor|].
     destruct (decode p) as [i|] eqn:?; simplify_eq/=; constructor; eauto.
@@ -122,7 +124,7 @@ Proof.
     feed pose proof (proj1 (Forall_forall _ _) Hm' (p',x')); simpl in *; auto.
     by destruct (decode p') as [i'|]; simplify_eq/=.
   - intros A [m Hm] i x; unfold map_to_list, lookup; simpl.
-    apply bool_decide_unpack in Hm; rewrite elem_of_list_omap; split.
+    apply sprop_decide_unpack in Hm; rewrite elem_of_list_omap; split.
     + intros ([p' x']&Hp'&?); apply elem_of_map_to_list in Hp'.
       feed pose proof (Hm p' x'); simpl in *; auto.
       by destruct (decode p') as [i'|] eqn:?; simplify_eq/=.
